src/OSum/binary_logrel.v
@@ -1,0 +1,73 @@
+From stdpp Require Import base gmap.
+
+From iris.base_logic Require Import invariants iprop upred saved_prop.
+From iris.base_logic.lib Require Import gset_bij .
+From iris.algebra Require Import gset_bij excl gmap.
+From iris.proofmode Require Import proofmode.
+From iris.program_logic Require Import weakestpre.
+Require Import Autosubst.Autosubst.
+
+From Equations Require Import Equations.
+
+From MyProject.src.OSum Require Export OSum persistent_pred wp_rules.
+
+Definition specN := nroot .@ "spec".
+
+
+
+Definition D `{Σ : gFunctors}:= persistent_pred (val * val) (iProp Σ).
+
+(* need to enhance state.. *)
+Class logrelSig  Σ := Resources {
+    invariants : invGS Σ;
+    predicates :: savedPredG Σ (val * val) ;
+    names :: gset_bijG Σ loc loc ;
+    name_set : gname
+}.
+Check rtc.
+Check erased_step. 
+Locate erased_step.
+Check gset_bijR.
+
+
+Definition combine (l1 l2 : list loc) : gset (loc * loc) := 
+    list_to_set (zip l1 l2).
+
+Definition spec_thread : cmra := exclR exprO.
+Definition configRA : cmra := prodR spec_thread (gset_bijR loc loc).
+
+Definition as_thread (e : expr) : spec_thread := Excl e.
+
+Class configSpec Σ := CS { 
+    config_in :: inG Σ configRA ; 
+    spec_predicates :: savedPredG Σ (val * val) ;
+    config_name : gname
+}.
+
+Section definitionsS.
+    Context `{configSpec Σ, invGS Σ}.
+    Definition spec_inv (ρ : cfg OSum_lang) : iProp Σ := 
+        (∃ e s s', own config_name (Excl e , ●V (combine s s'))
+                    ∗ [∗ list] l' ∈ s', (∃ (P : D), saved_pred_own l' (DfracDiscarded) P)
+                    ∗ ⌜rtc erased_step ρ ([e],s)⌝)%I.
+
+    Definition spec_ctx : iProp Σ :=
+        (∃ ρ, inv specN (spec_inv ρ))%I.
+    
+End definitionsS.
+
+
+
+Definition state_interp `{logrelSig Σ} (s : list loc) : iProp Σ :=
+    ∃ (s' : list loc ) , 
+            gset_bij_own_auth name_set (DfracOwn 1) (combine s s')  ∗
+            [∗ list] l' ∈ s', (∃ (P : D), saved_pred_own l' (DfracDiscarded) P).
+
+
+Global Instance OSum_irisGS `{logrelSig Σ} : irisGS OSum_lang Σ := {
+    iris_invGS := invariants;
+    num_laters_per_step _ := 0;
+    state_interp s  _ _ _ := state_interp s;
+    fork_post _ := True%I;
+    state_interp_mono _ _ _ _ := fupd_intro _ _
+}.
