src/OSum/unary_soundness.v
@@ -1,0 +1,134 @@
+
+From iris.proofmode Require Import proofmode.
+From iris.program_logic Require Import adequacy.
+From iris.prelude Require Import options.
+From iris.base_logic.lib Require Import gset_bij .
+Require Import Autosubst.Autosubst.
+
+From MyProject.src.OSum Require Export unary_fundamental.
+
+(*
+  "adequate" 
+      Record adequate {Λ} (s : stuckness) (e1 : expr Λ) (σ1 : state Λ)
+      (φ : val Λ → state Λ → Prop) := {
+        adequate_result t2 σ2 v2 :
+            rtc erased_step ([e1], σ1) (of_val v2 :: t2, σ2) → 
+            φ v2 σ2;
+        adequate_not_stuck t2 σ2 e2 :
+            s = NotStuck →
+            rtc erased_step ([e1], σ1) (t2, σ2) →
+            e2 ∈ t2 → 
+            not_stuck e2 σ2
+      }.
+
+      has two fields, (we only care about the second one for the moment)
+      stating that given any epression e1 and state σ1, 
+        whenever e1 with program state σ1 evaluates to an expression e2 with program state σ2
+        the program is not stuck
+          meaning e2 is either a value or it can be reduced further
+
+        where
+
+          Definition not_stuck (e : expr Λ) (σ : state Λ) :=
+            is_Some (to_val e) ∨ reducible e σ.
+          Definition reducible (e : expr Λ) (σ : state Λ) :=
+            ∃ κ e' σ' efs, prim_step e σ κ e' σ' efs.
+
+        Note that prim_step is the base reduction a user gives in the definition of "Language"
+
+  We want to show that any well typed OSum_lang program e with the empty program state [] 
+  is safe to evaluate.
+ *)
+
+Class capabilities Σ := Cap {
+  invs :: invGpreS Σ;
+  res :: RelationResources Σ ;
+}.
+
+(* Any execution of e starting in the empty program state should not become stuck.
+    I demand e start in an empty program state here.
+    e could start in an arbitrary program state s
+      in order to state this, we'd have to construct a ghost state from program state s
+      This would require additional information not in s, specifically |s| many predicates on "val"
+
+    In the case [] ⊢ₜ e : τ,
+      e is a closed term that can't use any predicates in the ghost state
+        it might as well be empty
+      The only syntactically well-typed way to introduce a case symbol is from the 
+      expression "New t" which is guarunteed to generate a case that is fresh.
+*)
+Definition safe (e : expr) := 
+  forall e' s', rtc erased_step ([e], []) ([e'], s') → not_stuck e' s'.
+
+Theorem adequacy_of_semantic_typing `{capabilities Σ}(e : expr) (t : type) : 
+  (∀ `{logrelSig Σ}, ⊢ [] ⊨ e : t) -> safe e.
+Proof.
+  intros semtyped.
+  (* adequacy of WP for OSum_lang is enough to prove this *)
+  enough (adequate NotStuck e [] (fun _ _ => True)) as [_ notStuck].
+  - (* assuming adequacy of WP for OSum_lang 
+      simply use the field "adequate_not_stuck" of "adequacy"  *)
+    unfold safe ;intros e' s' reduces. 
+    pose proof (notStuck [e'] s' e' eq_refl reduces).
+    apply H0.
+    apply elem_of_list_singleton.
+    done.
+  - (* Now we have to prove adequacy 
+    which via "wp_adequacy_gen", it is sufficient to show 
+    "state_interp [] ∗ WP e {{ _, True }}" *)
+  eapply wp_adequacy_gen; simpl.
+  + (* summon the invariant instance *)
+  apply _.
+  + intros Hinv ks.
+  (* allocate an empty type store *)
+  iMod (init_state) as "[%ts stInterp]".
+  iModIntro.
+  (* these have to be the same state_interp and fork_post used in the semantic typing proof 
+    otherwise the proof won't go through since the implicits to wp dont align.
+    You can see this if you set this flag and unfold definitions
+      Set Printing Implicit. 
+  *)
+  iExists (fun s _ =>state_interp s).
+  iExists (fun _ => True%I).
+  (* It is easy to prove the state_interp for the empty program state *)
+  iSplitL. { done. }
+  (*  to prove  WP e {{ _, True }}, we can just use ⊢ [] ⊨ e : t
+      this is because we can apply empty rho and empty gamma to  ⊢ [] ⊨ e : t 
+      which boils down to WP e {{ v, interp t [] v }},
+  *)
+  (* in order to use ⊢ [] ⊨ e : t 
+  we need to have a concrete instance of ghost state, logSigΣ 
+  we need to adjust the post condition,
+  and we need to massage e *)
+  set (logSigΣ := LogRelSig Σ Hinv ts).
+  replace e with e.[env_subst[]] by by asimpl.
+  iApply wp_wand. { 
+    (* just apply the fact that e is well typed *)
+  iApply (semtyped logSigΣ $! [] [] ). iApply interp_env_nil. }
+  eauto.
+Qed.
+ 
+(* what kind of typeclass magic is going on here? *)
+Definition gen_ResΣ : gFunctors := #[savedPredΣ val ; gset_bijΣ loc loc].
+
+Global Instance subG_ResΣ {Σ} : subG gen_ResΣ Σ → RelationResources Σ.
+Proof. solve_inG. Qed.
+
+Example foo : sigT RelationResources .
+set (Σ' := #[gen_ResΣ ]).
+exists Σ'.
+apply _.
+Qed.
+
+Corollary type_soundness e τ  :
+  [] ⊢ₜ e : τ → safe e.
+Proof.
+  intros ?. 
+  (* chose the exact gFunctors / capabilities, 
+  namely invariants, bijection, and saved pred *)
+  set (Σ := #[invΣ ; gen_ResΣ]). 
+  (* make a "capabilities Σ" instance to apply above result*)
+  set (C := (Cap Σ _ _)).
+  eapply (@adequacy_of_semantic_typing Σ C). 
+  intros. apply fundamental. exact H.
+Qed.
